high2/Zeta.High.Verifier.EAC.fst
@@ -1,11 +1,16 @@
 module Zeta.High.Verifier.EAC
 
+open Zeta.Interleave
 open Zeta.App
 open Zeta.Key
+open Zeta.GenKey
 open Zeta.Time
+open Zeta.MultiSet
 open Zeta.MultiSetHashDomain
 open Zeta.GenericVerifier
+open Zeta.Generic.Blum
 open Zeta.EAC
+open Zeta.High.Thread
 open Zeta.High.Interleave
 
 module S = FStar.Seq
@@ -13,6 +18,7 @@ module I = Zeta.Interleave
 module T = Zeta.Generic.Thread
 module G = Zeta.Generic.Global
 module GI=Zeta.Generic.Interleave
+module GB = Zeta.Generic.Blum
 module GTL=Zeta.Generic.TSLog
 module HI=Zeta.High.Interleave
 module HTL=Zeta.High.TSLog
@@ -37,21 +43,40 @@ let lemma_non_eac_init_addb
   (epmax: epoch)
   (itsl: neac_before_epoch app n epmax
     {let fi = eac_failure itsl in
-     GI.aems_equal_upto epmax itsl /\
+     GB.aems_equal_upto epmax itsl /\
      fi.es = EACInit /\
      AddB? fi.le})
+  : hash_collision app
   = let fi = eac_failure itsl in
-    let be = blum_add_elem itsl fi.bi in
+    let i = fi.bi in
+    let be = blum_add_elem itsl i in
+    let ep = be.t.e in
+    let itsli = prefix itsl i in
 
+    // since fi.es is EACInit, there cannot be a prior entry for fi.bk
+    //assert(eac_state_of_key fi.bk itsli = EACInit);
+    eac_state_init_implies_no_key_refs fi.bk itsli;
+    //assert(~ (has_some_ref_to_key fi.bk itsli));
 
+    if evict_set ep itsl `contains` be then (
+      (* if evict set contains be, then the index of be should be prior to i *)
+      let j = evict_elem_idx itsl be in
+      lemma_evict_before_add itsl i;
+      assert(j < i);
 
-
-    admit()
+      (* this implies a prior reference to fi.bk which is a contradiction *)
+      FStar.Classical.exists_intro (fun i -> refs_key (I.index itsli i) fi.bk) j;
+      hash_collision_contra app
+    )
+    else (
+      not_eq (add_set ep itsl) (evict_set ep itsl) be;
+      hash_collision_contra app
+    )
 
 let lemma_neac_implies_hash_collision
   (#app #n:_)
   (epmax: epoch)
-  (itsl: neac_before_epoch app n epmax {GI.aems_equal_upto epmax itsl})
+  (itsl: neac_before_epoch app n epmax {GB.aems_equal_upto epmax itsl})
   : hash_collision app
   = let fi = eac_failure itsl in
     eac_boundary_not_appfn itsl;
