generic/Zeta.Generic.Blum.fsti
@@ -1,0 +1,76 @@
+module Zeta.Generic.Blum
+
+open Zeta.Interleave
+open Zeta.MultiSet
+open Zeta.Time
+open Zeta.MultiSetHashDomain
+open Zeta.GenericVerifier
+open Zeta.Generic.Interleave
+open Zeta.Generic.TSLog
+
+module S = FStar.Seq
+module SA = Zeta.SeqAux
+module G = Zeta.Generic.Global
+
+val add_il (#vspec #n:_) (ep: epoch) (il: verifiable_log vspec n)
+  : interleaving (ms_hashfn_dom vspec.app) n
+
+let add_seq (#vspec #n:_) (ep: epoch) (il: verifiable_log vspec n)
+  : S.seq (ms_hashfn_dom vspec.app)
+  = i_seq (add_il ep il)
+
+let add_set #vspec #n (ep: epoch) (il: verifiable_log vspec n)
+  : mset_ms_hashfn_dom vspec.app
+  = seq2mset (add_seq ep il)
+
+val evict_il (#vspec #n:_) (ep: epoch) (il: verifiable_log vspec n)
+  : interleaving (ms_hashfn_dom vspec.app) n
+
+let evict_seq (#vspec #n:_) (ep: epoch) (il: verifiable_log vspec n)
+  : S.seq (ms_hashfn_dom vspec.app)
+  = i_seq (evict_il ep il)
+
+let evict_set #vspec #n (ep: epoch) (il: verifiable_log vspec n)
+  : mset_ms_hashfn_dom vspec.app
+  = seq2mset (evict_seq ep il)
+
+let aems_equal_upto #vspec #n (epmax: epoch) (il: verifiable_log vspec n)
+  = forall (ep: epoch). ep <= epmax ==> add_set ep il == evict_set ep il
+
+val lemma_add_evict_set_identical_glog (#vspec #n:_) (epmax: epoch) (il: verifiable_log vspec n)
+  : Lemma (ensures (aems_equal_upto epmax il <==> G.aems_equal_upto epmax (to_glog il)))
+
+val add_set_contains_each_add_elem (#vspec #n:_) (il: verifiable_log vspec n) (i: seq_index il{is_blum_add il i})
+  : Lemma (ensures (let be = blum_add_elem il i in
+                    let ep = be.t.e in
+                    add_set ep il `contains` be))
+          [SMTPat (blum_add_elem il i)]
+
+val some_add_elem_idx
+  (#vspec #n:_)
+  (il: verifiable_log vspec n)
+  (be: ms_hashfn_dom vspec.app {let ep = be.t.e in
+                                add_set ep il `contains` be})
+  : i: seq_index il {is_blum_add il i /\ be = blum_add_elem il i}
+
+val evict_set_contains_each_evict_elem (#vspec #n:_) (il: verifiable_log vspec n) (i: seq_index il{is_blum_evict il i})
+  : Lemma (ensures (let be = blum_evict_elem il i in
+                    let ep = be.t.e in
+                    evict_set ep il `contains` be))
+          [SMTPat (blum_evict_elem il i)]
+
+val evict_set_is_a_set (#vspec #n:_) (ep: epoch) (il: verifiable_log vspec n)
+  : Lemma (ensures (is_set (evict_set ep il)) )
+
+val evict_elem_idx
+  (#vspec #n:_)
+  (il: verifiable_log vspec n)
+  (be: ms_hashfn_dom vspec.app {let ep = be.t.e in
+                                evict_set ep il `contains` be})
+  : i: seq_index il {is_blum_evict il i /\ be = blum_evict_elem il i}
+
+val lemma_evict_before_add (#vspec #n:_) (itsl: its_log vspec n) (i:seq_index itsl{is_blum_add itsl i}):
+  Lemma (ensures (let be = blum_add_elem itsl i in
+                  let ep = be.t.e in
+                  not (evict_set ep itsl `contains` be) \/
+                  evict_elem_idx itsl be < i))
