high2/Zeta.High.Thread.fsti
@@ -1,0 +1,23 @@
+module Zeta.High.Thread
+
+open Zeta.GenKey
+open Zeta.GenericVerifier
+open Zeta.High.Verifier
+open Zeta.Generic.Thread
+
+let verifiable_log (app:_)
+  = Zeta.Generic.Thread.verifiable_log (high_verifier_spec app)
+
+val lemma_blum_add_elem_key (#app:_) (tl: verifiable_log app) (i: seq_index tl {is_blum_add tl i})
+  : Lemma (ensures (let open Zeta.MultiSetHashDomain in
+                    let be = blum_add_elem tl i in
+                    let gk,_ = be.r in
+                    add_slot (index tl i) = to_base_key gk))
+          [SMTPat (blum_add_elem tl i)]
+
+val lemma_blum_evict_elem_key (#app:_) (tl: verifiable_log app) (i: seq_index tl {is_blum_evict tl i})
+  : Lemma (ensures (let open Zeta.MultiSetHashDomain in
+                    let be = blum_evict_elem tl i in
+                    let gk,_ = be.r in
+                    evict_slot (index tl i) = to_base_key gk))
+          [SMTPat (blum_evict_elem tl i)]
