high2/Zeta.High.Verifier.EAC.fsti
@@ -8,9 +8,10 @@ open Zeta.High.Verifier
 open Zeta.High.TSLog
 
 module GI = Zeta.Generic.Interleave
+module GB = Zeta.Generic.Blum
 
 val lemma_neac_implies_hash_collision
   (#app #n:_)
   (epmax: epoch)
-  (itsl: neac_before_epoch app n epmax {GI.aems_equal_upto epmax itsl})
+  (itsl: neac_before_epoch app n epmax {GB.aems_equal_upto epmax itsl})
   : hash_collision app
